equational_theories/Definability.lean
@@ -160,6 +160,7 @@ import equational_theories.Definability.DiagRep03
 import equational_theories.Definability.DiagRep04
 import equational_theories.Definability.DiagRep05
 import equational_theories.Definability.DiagRep06
+import equational_theories.Definability.DiagB_00
 import equational_theories.Definability.UnaryFine463_0
 import equational_theories.Definability.UnaryFine463_1
 import equational_theories.Definability.Certs
